theories/Assoc.v
@@ -1,0 +1,21 @@
+Require Import Coq.Unicode.Utf8.
+Require Import Coq.Arith.PeanoNat.
+
+Require Import FunInd.
+
+Import IfNotations.
+
+Import Nat.
+
+Definition assoc (A: Set) := list (nat * A).
+
+Function find {A: Set} x (l: assoc A) :=
+  if l is ((y, t) :: T)%list
+  then
+    if Nat.eq_dec x y
+    then
+      Some t
+    else
+      find x T
+  else
+    None.
